feat: instantiateLevelParams proof

Lean4Lean/Theory/VLevel.lean
@@ -43,6 +43,15 @@ theorem le_refl (a : VLevel) : a ≤ a := fun _ => Nat.le_refl _
 theorem le_trans {a b c : VLevel} (h1 : a ≤ b) (h2 : b ≤ c) : a ≤ c :=
   fun _ => Nat.le_trans (h1 _) (h2 _)
 
+theorem zero_le : zero ≤ a := fun _ => Nat.zero_le _
+
+theorem le_succ : a ≤ succ a := fun _ => Nat.le_succ _
+
+theorem succ_le_succ (h : a ≤ b) : succ a ≤ succ b := fun _ => Nat.succ_le_succ (h _)
+
+theorem le_max_left : a ≤ max a b := fun _ => Nat.le_max_left ..
+theorem le_max_right : b ≤ max a b := fun _ => Nat.le_max_right ..
+
 protected def Equiv (a b : VLevel) : Prop := a.eval = b.eval
 
 instance : HasEquiv VLevel := ⟨VLevel.Equiv⟩
@@ -53,8 +62,35 @@ theorem equiv_def {a b : VLevel} : a ≈ b ↔ ∀ ls, a.eval ls = b.eval ls := 
 theorem le_antisymm_iff {a b : VLevel} : a ≈ b ↔ a ≤ b ∧ b ≤ a :=
   equiv_def.trans <| (forall_congr' fun _ => Nat.le_antisymm_iff).trans forall_and
 
-theorem succ_congr {a b : VLevel} (h : a ≈ b) : VLevel.succ a ≈ .succ b := by
+theorem succ_congr {a b : VLevel} (h : a ≈ b) : succ a ≈ succ b := by
   simpa [equiv_def, eval] using h
+
+theorem max_congr (h₁ : a₁ ≈ b₁) (h₂ : a₂ ≈ b₂) : max a₁ a₂ ≈ max b₁ b₂ := by
+  simp_all [equiv_def, eval]
+
+theorem imax_congr (h₁ : a₁ ≈ b₁) (h₂ : a₂ ≈ b₂) : imax a₁ a₂ ≈ imax b₁ b₂ := by
+  simp_all [equiv_def, eval]
+
+theorem max_comm : max a b ≈ max b a := by   simp [equiv_def, eval, Nat.max_comm]
+
+theorem LE.max_eq_left (h : b.LE a) : max a b ≈ a := by
+  simp [equiv_def, eval, Nat.max_eq_left (h _)]
+
+theorem LE.max_eq_right (h : a.LE b) : max a b ≈ b := by
+  simp [equiv_def, eval, Nat.max_eq_right (h _)]
+
+theorem max_self : max a a ≈ a := by simp [equiv_def, eval]
+
+theorem zero_imax : imax zero a ≈ a := by
+  simp [equiv_def, eval, Nat.imax, eq_comm (b := 0)]
+
+theorem imax_self : imax a a ≈ a := by
+  simp [equiv_def, eval, Nat.imax, eq_comm (b := 0)]
+
+def IsNeverZero (a : VLevel) : Prop := ∀ ls, a.eval ls ≠ 0
+
+theorem IsNeverZero.imax_eq_max (h : IsNeverZero b) : imax a b ≈ max a b := by
+  simp_all [equiv_def, eval, Nat.imax, IsNeverZero]
 
 variable (ls : List VLevel) in
 def inst : VLevel → VLevel
@@ -64,14 +100,14 @@ def inst : VLevel → VLevel
   | .imax l₁ l₂ => .imax l₁.inst l₂.inst
   | .param i => ls.getD i .zero
 
-theorem inst_inst {l : VLevel} : (l.inst ls).inst ls' = l.inst (ls.map (VLevel.inst ls')) := by
+theorem inst_inst {l : VLevel} : (l.inst ls).inst ls' = l.inst (ls.map (inst ls')) := by
   induction l <;> simp [inst, *, List.getD_eq_getElem?_getD, List.getElem?_map]
   case param n => cases ls[n]? <;> simp [inst]
 
 theorem inst_id {l : VLevel} (h : l.WF u) : l.inst ((List.range u).map .param) = l := by
   induction l <;> simp_all [inst, WF, List.getD_eq_getElem?_getD, List.getElem?_range]
 
-theorem eval_inst {l : VLevel} : (l.inst ls).eval ns = l.eval (ls.map (VLevel.eval ns)) := by
+theorem eval_inst {l : VLevel} : (l.inst ls).eval ns = l.eval (ls.map (eval ns)) := by
   induction l <;> simp [eval, inst, *, List.getD_eq_getElem?_getD]
   case param n => cases ls[n]? <;> simp [eval]
 
@@ -116,3 +152,8 @@ theorem WF.of_ofLevel (h : ofLevel ls l = some l') : l'.WF ls.length := by
   | succ _ ih => obtain ⟨l', h, ⟨⟩⟩ := h; exact @ih l' h
   | max _ _ ih1 ih2 | imax _ _ ih1 ih2 => obtain ⟨_, h1, _, h2, ⟨⟩⟩ := h; exact ⟨ih1 h1, ih2 h2⟩
   | param n => exact h.2 ▸ h.1
+
+theorem WF.of_mapM_ofLevel (h : List.mapM (VLevel.ofLevel Us) us = some us')
+    (a) (hl : a ∈ us') : VLevel.WF Us.length a := by
+  rw [List.mapM_eq_some] at h
+  have ⟨_, _, h⟩ := h.forall_exists_r _ hl; exact .of_ofLevel h
